minuska/theories/minusl_semantics.v
@@ -1,0 +1,65 @@
+From Minuska Require Import
+    prelude
+    spec_syntax
+    minusl_syntax
+    spec_semantics
+.
+
+
+Section MinusL_sem.
+    Context
+        {Σ : StaticModel}
+        (Act : Set)
+    .
+
+    Inductive MinusL_rewrites
+        (D : MinusL_LangDef Act)
+        :
+        (TermOver builtin_value) ->
+        (TermOver builtin_value) ->
+        (list Act)  ->
+        (TermOver builtin_value) ->
+        (TermOver builtin_value) ->
+        Prop :=
+
+    | mlr_rule : 
+        forall
+            (lc : TermOver BuiltinOrVar) (ld : TermOver BuiltinOrVar)
+            (a : Act)
+            (rc : TermOver Expression) (rd : TermOver Expression)
+            (scs : list SideCondition),
+            (mld_rewrite Act lc ld a rc rd scs) ∈ (mlld_decls Act D) ->
+        forall (ctrl1 state1 ctrl2 state2 : TermOver builtin_value)
+            (ρ : Valuation),
+            satisfies ρ ctrl1 lc ->
+            satisfies ρ state1 ld ->
+            satisfies ρ ctrl2 rc ->
+            satisfies ρ state2 rd ->
+            satisfies ρ () scs ->
+        MinusL_rewrites D ctrl1 state1 [a] ctrl2 state2
+
+    | mlr_trans :
+        forall
+            (ctrl1 state1 ctrl2 state2 ctrl3 state3 : TermOver builtin_value)
+            (w1 w2 : list Act),
+        MinusL_rewrites D ctrl1 state1 w1 ctrl2 state2 ->
+        MinusL_rewrites D ctrl2 state2 w2 ctrl3 state3 ->
+        MinusL_rewrites D ctrl1 state1 (w1 ++ w2) ctrl3 state3
+
+    | mlr_context :
+        forall
+            (c : TermOver BuiltinOrVar)
+            (h : variable)
+            (Hh : length (filter (eq h) (vars_of_to_l2r c)) = 1)
+            (scs : list SideCondition)
+            (Hhscs : h ∉ vars_of scs),
+            (mld_context Act c h Hh scs Hhscs) ∈ (mlld_decls Act D) ->
+        forall (ctrl1 state1 ctrl2 state2 r v : TermOver builtin_value)
+            (w : list Act),
+            (∃ (ρ1 : Valuation), satisfies (<[h := uglify' r]>ρ1) ctrl1 c /\ satisfies ρ1 () scs) ->
+            (∃ (ρ2 : Valuation), satisfies (<[h := uglify' v]>ρ2) ctrl2 c /\ satisfies ρ2 () (mlld_isValue Act D (ft_element (uglify' v)))) ->
+            MinusL_rewrites D r state1 w v state2 ->
+            MinusL_rewrites D ctrl1 state1 w ctrl2 state2
+    .
+
+End MinusL_sem.
