minuska/theories/minusl_syntax.v
@@ -1,0 +1,78 @@
+From stdpp Require Import finite.
+
+From Minuska Require Import
+    prelude
+    spec_syntax
+    varsof
+.
+
+
+
+Variant MinusL_Decl {Σ : StaticModel} (Act : Set) :=
+| mld_rewrite
+    (lc : TermOver BuiltinOrVar) (ld : TermOver BuiltinOrVar)
+    (a : Act)
+    (rc : TermOver Expression) (rd : TermOver Expression)
+    (scs : list SideCondition)
+| mld_context
+    (c : TermOver BuiltinOrVar)
+    (h : variable)
+    (Hh : length (filter (eq h) (vars_of_to_l2r c)) = 1)
+    (scs : list SideCondition)
+    (Hhscs : h ∉ vars_of scs)
+. 
+
+Definition actions_of_decl
+    {Σ : StaticModel}
+    (Act : Set)
+    (d : MinusL_Decl Act)
+    : list Act
+:=
+match d with
+| mld_rewrite _ _ _ a _ _ _ => [a]
+| mld_context _ _ _ _ _ _ => []
+end.
+
+
+Record MinusL_LangDef
+    {Σ : StaticModel}
+    (Act : Set)
+    : Type
+ := mkMinusL_LangDef {
+    mlld_isValue : Expression -> (list SideCondition) ;
+    mlld_decls : list (MinusL_Decl Act) ;
+}.
+
+
+Definition actions_of_ldef
+    {Σ : StaticModel}
+    (Act : Set)
+    (D : MinusL_LangDef Act)
+    : list Act
+:=
+    concat (map (actions_of_decl Act) (mlld_decls Act D))
+.
+
+
+#[export]
+Instance VarsOf_MinusL_Decl
+    {Σ : StaticModel}
+    (Act : Set)
+    : VarsOf (MinusL_Decl Act) variable
+:= {|
+    vars_of := fun D => match D with
+    | mld_rewrite _ lc ld _ rc rd scs => (vars_of lc) ∪ vars_of ld ∪
+        vars_of rc ∪ vars_of rd ∪ vars_of scs
+    | mld_context _ c h _ scs _ => (vars_of c) ∪ {[h]} ∪ vars_of scs
+    end ; 
+|}.
+
+#[export]
+Instance VarsOf_MinusL_LangDef
+    {Σ : StaticModel}
+    (Act : Set)
+    : VarsOf (MinusL_LangDef Act) variable
+:= {|
+    vars_of := fun D => union_list (vars_of <$> (mlld_decls Act D)) ; 
+|}.
+
