minuska/theories/varsof.v
@@ -166,26 +166,3 @@ Instance VarsOf_TermOverExpression
 := {|
     vars_of := fun t => vars_of (uglify' t)
 |}.
-
-#[export]
-Instance VarsOf_MinusL_Decl
-    {Σ : StaticModel}
-    (Act : Set)
-    : VarsOf (MinusL_Decl Act) variable
-:= {|
-    vars_of := fun D => match D with
-    | mld_rewrite _ lc ld _ rc rd scs => (vars_of lc) ∪ vars_of ld ∪
-        vars_of rc ∪ vars_of rd ∪ vars_of scs
-    | mld_context _ c h _ scs => (vars_of c) ∪ {[h]} ∪ vars_of scs
-    end ; 
-|}.
-
-#[export]
-Instance VarsOf_MinusL_LangDef
-    {Σ : StaticModel}
-    (Act : Set)
-    : VarsOf (MinusL_LangDef Act) variable
-:= {|
-    vars_of := fun D => union_list (vars_of <$> (mlld_decls Act D)) ; 
-|}.
-
